Added p3 prelude

Source/DafnyCore/Options/CommonOptionBag.cs
@@ -70,6 +70,14 @@ instantiations and suppressing major heap-wide propagation assumptions."
       IsHidden = true
     };
 
+  public static readonly Option<bool> Prelude3 =
+    new("--p3", () => false, @"
+(experimental) Load the third Boogie prelude variant, DafnyPrelude.p3.bpl.
+This can be used together with --qf-heap."
+      .TrimStart()) {
+      IsHidden = true
+    };
+
   public enum AssertionShowMode { None, Implicit, All }
   public static readonly Option<AssertionShowMode> ShowAssertions = new("--show-assertions", () => AssertionShowMode.None,
     "Show hints on locations where implicit assertions occur");
@@ -525,6 +533,8 @@ NoGhost - disable printing of functions, ghost methods, and proof
     DafnyOptions.RegisterLegacyUi(DefaultFunctionOpacity, DafnyOptions.ParseDefaultFunctionOpacity, "Language feature selection", "defaultFunctionOpacity", null);
     DafnyOptions.RegisterLegacyUi(QuantifierFreeFrames, DafnyOptions.ParseBoolean, "Verification options", "qfHeap", @"
 (experimental) Use the quantifier-light heap encoding mode.".TrimStart());
+    DafnyOptions.RegisterLegacyUi(Prelude3, DafnyOptions.ParseBoolean, "Verification options", "p3", @"
+(experimental) Load DafnyPrelude.p3.bpl.".TrimStart());
 
     DafnyOptions.RegisterLegacyUi(WarnContradictoryAssumptions, DafnyOptions.ParseImplicitEnable, "Verification options", "warnContradictoryAssumptions");
     DafnyOptions.RegisterLegacyUi(WarnRedundantAssumptions, DafnyOptions.ParseImplicitEnable, "Verification options", "warnRedundantAssumptions");
@@ -704,6 +714,7 @@ NoGhost - disable printing of functions, ghost methods, and proof
     OptionRegistry.RegisterOption(NoTimeStampForCoverageReport, OptionScope.Cli);
     OptionRegistry.RegisterOption(DefaultFunctionOpacity, OptionScope.Module);
     OptionRegistry.RegisterOption(QuantifierFreeFrames, OptionScope.Cli);
+    OptionRegistry.RegisterOption(Prelude3, OptionScope.Cli);
     OptionRegistry.RegisterOption(OptimizeErasableDatatypeWrapper, OptionScope.Cli); // TODO needs translation record registration
     OptionRegistry.RegisterOption(AddCompileSuffix, OptionScope.Cli);  // TODO needs translation record registration
     OptionRegistry.RegisterOption(SystemModule, OptionScope.Cli);
